formal-proofs/theories/lib/infinite_array/iterator.v
@@ -1,0 +1,149 @@
+From iris.heap_lang Require Import proofmode notation lang.
+Require Import SegmentQueue.lib.infinite_array.infinite_array_impl.
+
+Section impl.
+
+Variable segment_size: positive.
+
+Definition iterator_step: val :=
+  (λ: "seg" "idx",
+   let: "segv" := !"seg" in
+   let: "p" := FAA "idx" #1%nat in
+   let: "s" := (find_segment segment_size)
+                 "segv" ("p" `quot` #(Pos.to_nat segment_size)) in
+   ("s", "p" `rem` #(Pos.to_nat segment_size))).
+
+Definition increase_value_to: val :=
+  (λ: "loc" "val",
+     let: "tmp" := ref !"loc" in
+    (rec: "loop" <> :=
+       if: "tmp" < "val"
+       then if: CAS "loc" "tmp" "val" then #()
+            else "tmp" <- !"loc" ;; "loop" #()
+       else #()) #()
+  ).
+
+Definition iterator_step_skipping_cancelled: val :=
+  (rec: "loop" "seg" "idx" :=
+     let: "segv" := !"seg" in
+     let: "p" := FAA "idx" #1%nat in
+     let: "id" := ("p" `quot` #(Pos.to_nat segment_size)) in
+     let: "s" := (find_segment segment_size) "segv" "id" in
+     if: segment_id "s" = "id" then ("s", "p" `rem` #(Pos.to_nat segment_size))
+     else
+       increase_value_to "idx" (segment_id "s" * #(Pos.to_nat segment_size)) ;;
+       "loop" "seg" "idx"
+  ).
+
+End impl.
+
+From iris.program_logic Require Import atomic.
+From iris.algebra Require Import cmra auth list agree csum excl gset frac.
+
+Section proof.
+
+Context `{heapG Σ}.
+
+Variable ap: @infinite_array_parameters Σ.
+Let segment_size := p_segment_size ap.
+
+Variable cell_is_processed: nat -> iProp Σ.
+Variable cell_is_processed_persistent:
+  forall n, Persistent (cell_is_processed n).
+Existing Instance cell_is_processed_persistent.
+
+Context `{iArrayG Σ}.
+
+Notation algebra := (authR (gset_disjUR nat)).
+
+Class iteratorG Σ := IIteratorG { iterator_inG :> inG Σ algebra }.
+Definition iteratorΣ : gFunctors := #[GFunctor algebra].
+Instance subG_iteratorΣ {Σ} : subG iteratorΣ Σ -> iteratorG Σ.
+Proof. solve_inG. Qed.
+
+Context `{iteratorG Σ}.
+
+Notation iProp := (iProp Σ).
+
+Definition is_iterator γa γ fℓ ℓ: iProp :=
+  (∃ (n: nat), fℓ ↦ #n ∗ own γ (● (GSet (set_seq 0 n))) ∗
+                  ∃ (id: nat), ⌜(id * Pos.to_nat segment_size <= n)%nat⌝ ∗
+                                (∃ (ℓ': loc), segment_location γa id ℓ'
+                                                               ∗ ℓ ↦ #ℓ'))%I.
+
+Lemma quot_of_nat n m:
+  Z.of_nat n `quot` Z.of_nat m = Z.of_nat (n `div` m).
+Proof.
+  destruct m. destruct n; done.
+  rewrite Z2Nat_inj_div; apply Z.quot_div_nonneg; lia.
+Qed.
+
+Lemma rem_of_nat n m:
+  Z.of_nat n `rem` Z.of_nat (S m) = Z.of_nat (n `mod` S m).
+Proof.
+  rewrite Z2Nat_inj_mod; apply Z.rem_mod_nonneg; lia.
+Qed.
+
+Theorem iterator_step_spec γa γ (ℓ fℓ: loc):
+  cell_init ap -∗
+  <<< ▷ is_infinite_array ap γa ∗ is_iterator γa γ fℓ ℓ >>>
+    (iterator_step segment_size) #ℓ #fℓ @ ⊤
+    <<< ∃ (ix: nat) (sℓ: loc),
+      ▷ is_infinite_array ap γa ∗ is_iterator γa γ fℓ ℓ ∗
+      ∃ (id: nat) (n: nat),
+      ⌜(ix < Pos.to_nat segment_size)%nat⌝ ∗
+      ⌜(id * Pos.to_nat segment_size <= n)%nat⌝ ∗
+      segment_location γa id sℓ ∗
+      own γ (◯ (GSet {[ n ]})) ∗
+      (∃ ℓ, p_cell_invariant ap γa (id * Pos.to_nat segment_size + ix) ℓ) ∗
+      (⌜n = (id * Pos.to_nat segment_size + ix)%nat⌝ ∨ cell_is_cancelled' γa id ix),
+           RET (#sℓ, #ix) >>>.
+Proof.
+  iIntros "#HCellInit".
+  iIntros (Φ) "AU". wp_lam. wp_pures.
+
+  wp_bind (!_)%E.
+  iMod "AU" as "[[HInfArr HIsIter] [HClose _]]".
+  iDestruct "HIsIter" as (?) "(Hfℓ & HAuth & HSeg)".
+  iDestruct "HSeg" as (? ? ?) "(#HSegLoc & Hℓ)".
+  wp_load.
+  iMod ("HClose" with "[-]") as "AU". {
+    rewrite /is_iterator. repeat (iFrame; iExists _).
+    iSplitR. 2: by iExists _; iFrame. done.
+  }
+  iModIntro. wp_pures.
+
+  wp_bind (FAA _ _)%E.
+  iMod "AU" as "[[HInfArr HIsIter] [HClose _]]".
+  iDestruct "HIsIter" as (n) "(Hfℓ & HAuth & HSeg)".
+  iDestruct "HSeg" as (? ? ?) "(#HSegLoc' & Hℓ)".
+  wp_faa.
+  iMod (own_update with "HAuth") as "[HAuth HFrag]".
+  { apply auth_update_alloc.
+    eapply (gset_disj_alloc_empty_local_update _ {[ n ]}).
+    apply (set_seq_S_end_disjoint 0). }
+  rewrite -(set_seq_S_end_union_L 0).
+  iMod ("HClose" with "[-]") as "AU". {
+    rewrite /is_iterator. iFrame; repeat (iExists _; iFrame).
+    replace (n + 1%nat) with (Z.of_nat (S n)) by lia. iFrame.
+    iExists _; iFrame.
+    iSplitR. 2: by iExists _; iFrame. iPureIntro. lia.
+  }
+  iModIntro. wp_pures.
+
+  wp_bind (find_segment _ _ _).
+  replace (Z.of_nat n `quot` Z.of_nat (Pos.to_nat segment_size)) with
+      (Z.of_nat (n `div` Pos.to_nat segment_size)%nat).
+  2: by rewrite quot_of_nat.
+
+  awp_apply find_segment_spec; try done.
+  iApply (aacc_aupd_commit with "AU"); first done.
+  iIntros "[HInfArr HIsIter]".
+  iAaccIntro with "HInfArr".
+  { iIntros "HInfArr". iFrame. eauto. }
+
+  iIntros (? ?) "(HInfArr & HSegInv & #HSegLoc'' & HFindSegRet)".
+
+  iDestruct "HFindSegRet" as "[[% ->]|(% & % & #HCanc)]".
+
+Abort.
